michael_formal/EFSM_LTL.thy
@@ -1,42 +1,39 @@
 theory EFSM_LTL
-imports EFSM "~~/src/HOL/Library/Linear_Temporal_Logic_on_Streams" Filesystem
+imports EFSM "~~/src/HOL/Library/Linear_Temporal_Logic_on_Streams"
 begin
 
-record state =
-  statename :: "statename option"
+record 'statename state =
+  statename :: "'statename option"
   datastate :: datastate
   event :: event
   "output" :: outputs
 
-type_synonym full_observation = "state stream"
-type_synonym property = "full_observation \<Rightarrow> bool"
+type_synonym 'statename full_observation = "'statename state stream"
+type_synonym 'statename property = "'statename full_observation \<Rightarrow> bool"
 
-abbreviation label :: "state \<Rightarrow> string" where
+abbreviation label :: "'statename state \<Rightarrow> string" where
   "label s \<equiv> fst (event s)"
 
-abbreviation inputs :: "state \<Rightarrow> value list" where
+abbreviation inputs :: "'statename state \<Rightarrow> value list" where
   "inputs s \<equiv> snd (event s)"
 
-fun ltl_step :: "efsm \<Rightarrow> statename option \<Rightarrow> datastate \<Rightarrow> event \<Rightarrow> (statename option \<times> outputs \<times> datastate)" where
-"ltl_step _ None r _ = (None, [], r)" |
-"ltl_step e (Some s) r (l, i) = (case (possible_steps e s r l i) of
-    [(s',t)] \<Rightarrow> (Some s', (apply_outputs (Outputs t) (join_ir i r)), (apply_updates (Updates t) (join_ir i r) r)) |
-    _ \<Rightarrow> (None, [], r)
-  )"
+fun ltl_step :: "'statename efsm \<Rightarrow> 'statename option \<Rightarrow> datastate \<Rightarrow> event \<Rightarrow> ('statename option \<times> outputs \<times> datastate)" where
+  "ltl_step _ None r _ = (None, [], r)" |
+  "ltl_step e (Some s) r (l, i) = (if is_singleton (possible_steps e s r l i) then (let (s', t) =  (the_elem (possible_steps e s r l i)) in (Some s', (apply_outputs (Outputs t) (join_ir i r)), (apply_updates (Updates t) (join_ir i r) r))) else (None, [], r))"
 
-primcorec make_full_observation :: "efsm \<Rightarrow> statename option \<Rightarrow> datastate \<Rightarrow> event stream \<Rightarrow> full_observation" where
+primcorec make_full_observation :: "'statename efsm \<Rightarrow> 'statename option \<Rightarrow> datastate \<Rightarrow> event stream \<Rightarrow> 'statename full_observation" where
   "make_full_observation e s d i = (let (s', o', d') = ltl_step e s d (shd i) in \<lparr>statename = s, datastate = d, event=(shd i), output = o'\<rparr>##(make_full_observation e s' d' (stl i)))"
 
-abbreviation non_null :: property where
+abbreviation non_null :: "'statename property" where
   "non_null s \<equiv> (statename (shd s) \<noteq> None)"
 
-abbreviation null :: property where
+abbreviation null :: "'statename property" where
   "null s \<equiv> (statename (shd s) = None)"
 
 lemma null_forever [simp]: "s = make_full_observation e (Some (s0 e)) <> t \<Longrightarrow> null s \<Longrightarrow> nxt (alw null) s"
   by simp
 
-abbreviation some_state :: "full_observation \<Rightarrow> bool" where
+abbreviation some_state :: "'statename full_observation \<Rightarrow> bool" where
   "some_state s \<equiv> (\<exists>state. statename (shd s) = Some state)"
 
 lemma non_null_equiv: "non_null = some_state"
@@ -55,7 +52,4 @@ proof (coinduction)
   then show ?case
     by (smt UNTIL.coinduct non_null_equiv)
 qed
-
-
-
 end
