michael_formal/drinks_machine_change.thy
@@ -11,16 +11,19 @@ definition vend :: "transition" where
         Updates = [(R 1, (V (R 1))), (R 2, (V (R 2)))]
       \<rparr>"
 
-definition drinks :: "efsm" where
+definition drinks :: "drinks_machine.statename efsm" where
 "drinks \<equiv> \<lparr> 
-          S = [1,2,3],
-          s0 = 1,
+          s0 = q1,
           T = \<lambda> (a,b) .
-              if (a,b) = (1,2) then [select] (* If we want to go from state 1 to state 2 then select will do that *)
-              else if (a,b) = (2,2) then [coin] (* If we want to go from state 2 to state 2 then coin will do that *)
-              else if (a,b) = (2,3) then [vend] (* If we want to go from state 2 to state 3 then drinks will do that *)
-              else [] (* There are no other transitions *)
+                   if (a,b) = (q1,q2) then {select} (* If we want to go from state 1 to state 2 then select will do that *)
+              else if (a,b) = (q2,q2) then {coin} (* If we want to go from state 2 to state 2 then coin will do that *)
+              else if (a,b) = (q2,q3) then {vend} (* If we want to go from state 2 to state 3 then drinks will do that *)
+              else {} (* There are no other transitions *)
          \<rparr>"
+
+lemma s0_drinks [simp]: "s0 drinks = q1"
+  by (simp add: drinks_def)
+
 
 (*
   These are lemmas about the machine which could maybe be in another file.
@@ -32,30 +35,81 @@ lemmas transitions = select_def coin_def vend_def
 lemma "observe_trace drinks (s0 drinks) <> [] = []"
   by simp
 
+lemma label_select_q2: "Label b = ''select'' \<Longrightarrow> b \<in> T drinks_machine_change.drinks (q1, a) \<Longrightarrow> b = select \<and> a = q2"
+  apply (simp add: drinks_def)
+  apply (cases a)
+  by simp_all
+
+lemma possible_steps_q1: "possible_steps drinks q1 Map.empty ''select'' [Str ''coke''] = {(q2, select)}"
+  apply (simp add: possible_steps_def)
+  apply safe
+       apply (simp add: label_select_q2)
+      apply (simp add: label_select_q2)
+     apply (simp add: select_def)
+    apply (simp add: drinks_def)
+   apply (simp add: select_def)
+  by (simp add: select_def)
+
 lemma "observe_trace drinks (s0 drinks) <> [(''select'', [Str ''coke''])] = [[]]"
-  by (simp add: drinks_def transitions step_def)
+  by (simp add: possible_steps_q1)
 
-lemma "observe_trace drinks (s0 drinks) <> [(''select'', [Str ''coke'']), (''coin'', [Num 50])] = [[], [Num 50]]"
-  by (simp_all add: step_def drinks_def transitions)
+lemma label_coin_q2: "Label b = ''coin'' \<Longrightarrow> b \<in> T drinks (q2, a) \<Longrightarrow> b = coin \<and> a = q2"
+  apply (simp add: drinks_def)
+  apply (cases a)
+  by (simp_all add: vend_def)
 
-lemma "observe_trace drinks (s0 drinks) <> [(''select'', [Str ''coke'']), (''coin'', [Num 50]), (''coin'', [Num 50])] = [[], [Num 50], [Num 100]]"
-  by (simp add: step_def drinks_def transitions)
+lemma possible_steps_q2_coin: "possible_steps drinks q2 r ''coin'' [Num n'] = {(q2, coin)}"
+    apply (simp add: possible_steps_def)
+  apply safe
+       apply (simp add: label_coin_q2)
+      apply (simp add: label_coin_q2)
+     apply (simp add: coin_def)
+    apply (simp add: drinks_def coin_def)
+   apply (simp add: coin_def)
+  by (simp add: coin_def)
+
+lemma label_vend_q3: "Label b = ''vend'' \<Longrightarrow> b \<in> T drinks (q2, a) \<Longrightarrow> b = vend \<and> a = q3"
+  apply (simp add: drinks_def)
+  apply (cases a)
+  by (simp_all add: coin_def)
+
+lemma possible_steps_q2_vend: "n \<ge> 100 \<Longrightarrow> possible_steps drinks_machine_change.drinks q2 <R (Suc 0) := Str ''coke'', R 2 := Num n> ''vend'' [] = {(q3, vend)}"
+  apply (simp add: possible_steps_def)
+  apply safe
+       apply (simp add: label_vend_q3)
+      apply (simp add: label_vend_q3)
+     apply (simp add: vend_def)
+    apply (simp add: vend_def drinks_def)
+   apply (simp add: vend_def)
+  by (simp add: vend_def)
+
+lemma updates_coin_150 [simp]: "(apply_updates (Updates coin)
+          (case_vname (\<lambda>n. if n = Suc 0 then Some (Num 100) else index2state [] (Suc 0 + 1) (I n)) (\<lambda>n. if n = 2 then Some (Num 50) else <R (Suc 0) := Str ''coke''> (R n)))
+          <R (Suc 0) := Str ''coke'', R 2 := Num 50>) = <R 1 := Str ''coke'', R 2 := Num 150>"
+  apply (rule ext)
+  by (simp add: coin_def)
 
 lemma "observe_trace drinks (s0 drinks) <> [(''select'', [Str ''coke'']), (''coin'', [Num 50]), (''coin'', [Num 50]), (''vend'', [])] = [[], [Num 50], [Num 100], [Str ''coke'', Num 0]]"
-  by (simp_all add: step_def drinks_def transitions)
+  apply (simp add: possible_steps_q1 possible_steps_q2_coin possible_steps_q2_vend)
+  by (simp add: transitions)
 
 lemma "observe_trace drinks (s0 drinks) <> [(''select'', [Str ''coke'']), (''coin'', [Num 50]), (''coin'', [Num 100]), (''vend'', [])] = [[], [Num 50], [Num 150], [Str ''coke'', Num 50]]"
-  by (simp_all add: step_def drinks_def transitions)
+  apply (simp add: possible_steps_q1 possible_steps_q2_coin possible_steps_q2_vend)
+  by (simp add: transitions)
+
+lemma cat_impossible: "possible_steps drinks q2 <R (Suc 0) := Str ''coke'', R 2 := Num 0> ''cat'' [Num 50] = {}"
+  apply (simp add: possible_steps_def drinks_def)
+  by (simp add: vend_def coin_def)
 
 (*Stop when we hit a spurious input*)
 lemma "observe_trace drinks (s0 drinks) <> [(''select'', [Str ''coke'']), (''cat'', [Num 50])] = [[]]"
-  by (simp add: step_def drinks_def transitions)
+  by (simp add: possible_steps_q1 cat_impossible is_singleton_def)
 
 lemma "\<not> (valid_trace (drinks) [(''select'', [Str ''coke'']), (''cat'', [Num 50])])"
-  by(simp add: step_def drinks_def transitions)
+  by (simp add: possible_steps_q1 cat_impossible is_singleton_def)
 
 lemma "observe_trace drinks (s0 drinks) <> [(''select'', [Str ''coke'']), (''cat'', [Num 50]), (''coin'', [Num 50])] = [[]]"
-  by (simp add: step_def drinks_def transitions)
+  by (simp add: possible_steps_q1 cat_impossible is_singleton_def)
 
 lemma "( t = []) \<Longrightarrow> (observe_trace e (s0 e) <> t = []) "
   by(simp)
