michael_formal/drinks_machine_payforward.thy
@@ -1,5 +1,5 @@
 theory drinks_machine_payforward
-  imports EFSM CExp
+  imports EFSM CExp drinks_machine
 begin
 
 (* This version of drinks_machine supercedes all of those before 03/04/18 *)
@@ -11,12 +11,10 @@ definition "setup" :: "transition" where
         Arity = 0,
         Guard = [], (* No guards *)
         Outputs = [],
-        Updates = [ (* Two updates: *)
-                    (R 2, (L (Num 0)))
-                  ]
+        Updates = [(R 2, (L (Num 0)))]
       \<rparr>"
 
-definition "t1 \<equiv> \<lparr>
+definition "select1 \<equiv> \<lparr>
         Label = ''select'',
         Arity = 1,
         Guard = [], (* No guards *)
@@ -27,20 +25,8 @@ definition "t1 \<equiv> \<lparr>
                   ]
       \<rparr>"
 
-definition t2 :: "transition" where
-"t2 \<equiv> \<lparr>
-        Label = ''coin'',
-        Arity = 1,
-        Guard = [], (* No guards *)
-        Outputs = [(Plus (V (R 2)) (V (I 1)))], (* This could also be written infix with ''+'' *)
-        Updates = [
-                    (R 1, (V (R 1))), (* The value of r1 is unchanged *)
-                    (R 2, (Plus (V (R 2)) (V (I 1)))) (* The value of r2 is increased by the value of i1 *)
-                  ]
-      \<rparr>"
-
-definition t3 :: "transition" where
-"t3 \<equiv> \<lparr>
+definition vend :: "transition" where
+"vend \<equiv> \<lparr>
         Label = ''vend'',
         Arity = 0,
         Guard = [(Ge (V (R 2)) (L (Num 100)))], (* This is syntactic sugar for ''Not (Lt (V (R 2)) (N 100))'' which could also appear *)
@@ -51,20 +37,123 @@ definition t3 :: "transition" where
                   ]
       \<rparr>"
 
-definition vend :: "efsm" where
-"vend \<equiv> \<lparr> 
-          S = [1,2,3],
-          s0 = 1,
+definition drinks :: "drinks_machine.statename efsm" where
+"drinks \<equiv> \<lparr> 
+          s0 = q1,
           T = \<lambda> (a,b) .
-              if (a,b) = (1,2) then [setup] (* If we want to go from state 1 to state 2 then t1 will do that *)
-              else if (a,b) = (2,3) then [t1] (* If we want to go from state 2 to state 2 then t2 will do that *)
-              else if (a,b) = (3,3) then [t2] (* If we want to go from state 2 to state 3 then t3 will do that *)
-              else if (a,b) = (3,2) then [t3]
-              else [] (* There are no other transitions *)
+                   if (a,b) = (q1,q2) then {setup} (* If we want to go from state 1 to state 2 then select will do that *)
+              else if (a,b) = (q2,q3) then {select1} (* If we want to go from state 2 to state 2 then coin will do that *)
+              else if (a,b) = (q3,q3) then {coin} (* If we want to go from state 2 to state 3 then drinks will do that *)
+              else if (a,b) = (q3,q2) then {vend} (* If we want to go from state 2 to state 3 then drinks will do that *)
+              else {} (* There are no other transitions *)
          \<rparr>"
 
-lemmas transitions = t1_def t2_def t3_def setup_def
+lemma s0_drinks [simp]: "s0 drinks = q1"
+  by (simp add: drinks_def)
 
-lemma "observe_trace vend (s0 vend) <> [(''setup'', []), (''select'', [Str ''coke'']), (''coin'',[Num 110]), (''vend'', []), (''select'', [Str ''pepsi'']), (''coin'',[Num 90]), (''vend'', [])] = [[],[],[Num 110],[Str ''coke''],[],[Num 100],[Str ''pepsi'']]"
-  by (simp add: step_def vend_def transitions)
+lemmas transitions = select1_def coin_def vend_def setup_def
+
+lemma label_setup_q2: "Label b = ''setup'' \<Longrightarrow> b \<in> T drinks (q1, a) \<Longrightarrow> b = setup \<and> a = q2"
+  apply (simp add: drinks_def)
+  apply (cases a)
+  by simp_all
+
+lemma possible_steps_q1: "possible_steps drinks q1 Map.empty ''setup'' [] = {(q2, setup)}"
+  apply (simp add: possible_steps_def)
+  apply safe
+       apply (simp add: label_setup_q2)
+      apply (simp add: label_setup_q2)
+     apply (simp add: setup_def)
+    apply (simp add: drinks_def)
+   apply (simp add: setup_def)
+  by (simp add: setup_def)
+
+lemma apply_updates_setup [simp]: "(apply_updates (Updates setup) (case_vname Map.empty Map.empty) Map.empty) = <R 2 := Num 0>"
+  apply (simp add: setup_def)
+  apply (rule ext)
+  by simp
+
+lemma label_select_q2: "Label b = ''select'' \<Longrightarrow> b \<in> T drinks (q2, a) \<Longrightarrow> b = select1 \<and> a = q3"
+  apply (simp add: drinks_def)
+  apply (cases a)
+    apply simp
+   apply simp
+  by (simp add: select1_def)
+
+lemma possible_steps_q2: "possible_steps drinks_machine_payforward.drinks q2 d ''select'' [Str s] = {(q3, select1)}"
+  apply (simp add: possible_steps_def)
+  apply safe
+       apply (simp add: label_select_q2)
+      apply (simp add: label_select_q2)
+     apply (simp add: select1_def)
+    apply (simp add: select1_def drinks_def)
+   apply (simp add: select1_def)
+  by (simp add: select1_def)
+
+lemma updates_select1: "(apply_updates (Updates select1) (case_vname (\<lambda>n. if n = 1 then Some (Str d) else index2state [] (1 + 1) (I n)) (\<lambda>n. if n = 2 then Some (Num n') else None))
+          <R 2 := Num 0>) = <R 1 := Str d, R 2 := Num n'>"
+  apply (simp add: select1_def)
+  apply (rule ext)
+  by simp
+
+lemma label_coin_q3: "Label b = ''coin'' \<Longrightarrow> b \<in> T drinks_machine_payforward.drinks (q3, a) \<Longrightarrow> b = coin \<and> a = q3"
+  apply (simp add: drinks_def)
+  apply (cases a)
+    apply (simp add: vend_def)
+   apply (simp add: vend_def)
+  by (simp add: select1_def)
+
+lemma apply_updates_coin [simp]: "(apply_updates (Updates coin)
+          (case_vname (\<lambda>n. if n = 1 then Some (Num input) else index2state [] (1 + 1) (I n)) (\<lambda>n. if n = 2 then Some (Num original) else <R 1 := Str s> (R n)))
+          <R 1 := Str s, R 2 := Num original>) = <R 1 := Str s, R 2 := Num (original+input)>"
+  apply (simp add: coin_def)
+  apply (rule ext)
+  by simp
+
+lemma possible_steps_q3_coin: "possible_steps drinks_machine_payforward.drinks q3 d ''coin'' [Num n] = {(q3, coin)}"
+  apply (simp add: possible_steps_def)
+  apply safe
+       apply (simp add: label_coin_q3)
+      apply (simp add: label_coin_q3)
+     apply (simp add: coin_def)
+    apply (simp add: coin_def drinks_def)
+   apply (simp add: coin_def)
+  by (simp add: coin_def)
+
+lemma label_vend_q1: "Label b = ''vend'' \<Longrightarrow> b \<in> T drinks (q3, a) \<Longrightarrow> b = vend \<and> a = q2"
+  apply (simp add: drinks_def)
+  apply (cases a)
+    apply simp
+   apply simp
+  by (simp add: coin_def)
+
+lemma possible_steps_q3_vend: "n \<ge> 100 \<Longrightarrow> possible_steps drinks_machine_payforward.drinks q3 <R 1 := Str s, R 2 := Num n> ''vend'' [] = {(q2, vend)}"
+  apply (simp add: possible_steps_def)
+  apply safe
+       apply (simp add: label_vend_q1)
+      apply (simp add: label_vend_q1)
+     apply (simp add: vend_def)
+    apply (simp add: vend_def drinks_def)
+   apply (simp add: vend_def)
+  by (simp add: vend_def)
+
+lemma apply_updates_vend [simp]: "(apply_updates (Updates drinks_machine_payforward.vend) (case_vname Map.empty (\<lambda>n. if n = 2 then Some (Num 110) else <R 1 := Str ''coke''> (R n)))
+          <R 1 := Str ''coke'', R 2 := Num 110>) = <R 1 := Str ''coke'', R 2 := Num 10>"
+  apply (rule ext)
+  by (simp add: vend_def)
+
+lemma apply_updates_coin_2 [simp]:"(apply_updates (Updates coin)
+          (case_vname (\<lambda>n. if n = 1 then Some (Num 90) else index2state [] (1 + 1) (I n))
+            (\<lambda>n. apply_updates (Updates select1)
+                   (case_vname (\<lambda>n. if n = 1 then Some (Str ''pepsi'') else index2state [] (1 + 1) (I n)) (\<lambda>n. if n = 2 then Some (Num 10) else <R 1 := Str ''coke''> (R n)))
+                   <R 1 := Str ''coke'', R 2 := Num 10> (R n)))
+          (apply_updates (Updates select1)
+            (case_vname (\<lambda>n. if n = 1 then Some (Str ''pepsi'') else index2state [] (1 + 1) (I n)) (\<lambda>n. if n = 2 then Some (Num 10) else <R 1 := Str ''coke''> (R n)))
+            <R 1 := Str ''coke'', R 2 := Num 10>)) = <R 1 := Str ''pepsi'', R 2 := Num 100>"
+  apply (rule ext)
+  by (simp add: coin_def select1_def)
+
+lemma "observe_trace drinks (s0 drinks) <> [(''setup'', []), (''select'', [Str ''coke'']), (''coin'',[Num 110]), (''vend'', []), (''select'', [Str ''pepsi'']), (''coin'',[Num 90]), (''vend'', [])] = [[],[],[Num 110],[Str ''coke''],[],[Num 100],[Str ''pepsi'']]"
+  apply (simp add: possible_steps_q1 possible_steps_q2 updates_select1 possible_steps_q3_coin possible_steps_q3_vend del: One_nat_def)
+  by (simp add: transitions)
 end
